refinedVST/typing/globals.v
@@ -1,5 +1,7 @@
+Set Warnings "-notation-overridden,-custom-entry-overridden,-hiding-delimiting-key".
 From VST.typing Require Export type.
 From VST.typing Require Import programs.
+Set Warnings "notation-overridden,custom-entry-overridden,hiding-delimiting-key".
 From VST.typing Require Import type_options.
 
 Record global_type `{!typeG OK_ty Σ} {cs : compspecs} := GT {
