veric/simple_mapsto.v
@@ -1,0 +1,678 @@
+Require Import VST.veric.base.
+Set Warnings "-notation-overridden,-custom-entry-overridden,-hiding-delimiting-key".
+Require Import VST.veric.res_predicates.
+Set Warnings "notation-overridden,custom-entry-overridden,hiding-delimiting-key".
+Require Import VST.veric.juicy_mem.
+Require Import VST.veric.assert_lemmas.
+Require Import compcert.cfrontend.Ctypes.
+Require Import VST.veric.address_conflict.
+Require Import VST.veric.val_lemmas.
+Require Import VST.veric.Cop2.
+Require Import VST.veric.shares.
+Require Import VST.veric.slice.
+Require Import VST.veric.mpred.
+Require Import VST.veric.log_normalize.
+Require Import VST.veric.expr.
+Require Import VST.veric.juicy_mem_lemmas.
+Require Import VST.veric.mapsto_memory_block.
+Require Import VST.veric.valid_pointer.
+
+Section mpred.
+
+Context `{!heapGS Σ}.
+
+Definition mapsto (sh: Share.t) (t: type) (v1 v2 : val): mpred :=
+  match access_mode t with
+  | By_value ch =>
+   match type_is_volatile t with
+   | false =>
+    match v1 with
+     | Vptr b ofs =>
+       if readable_share_dec sh
+       then ⌜tc_val' t v2⌝ ∧ address_mapsto ch v2 sh (b, Ptrofs.unsigned ofs)
+       else ⌜tc_val' t v2 /\ (align_chunk ch | Ptrofs.unsigned ofs)⌝ ∧ nonlock_permission_bytes sh (b, Ptrofs.unsigned ofs) (size_chunk ch)
+     | _ => False
+    end
+    | _ => False
+    end
+  | _ => False
+  end.
+
+Definition mapsto_ sh t v1 := ∃ v, mapsto sh t v1 v.
+
+Lemma mapsto_tc_val': forall sh t p v, mapsto sh t p v ⊢ ⌜tc_val' t v⌝.
+Proof.
+  intros.
+  unfold mapsto.
+  destruct (access_mode t); auto.
+  if_tac; auto;
+  destruct p; auto;
+  try simple_if_tac; auto.
+  + iIntros "[$ _]".
+  + iIntros "[[$ _] _]".
+Qed.
+
+Lemma mapsto_weaken: forall sh t p v, mapsto sh t p v ⊢ mapsto_memory_block.mapsto sh t p v.
+Proof.
+  intros; rewrite /mapsto /mapsto_memory_block.mapsto.
+  destruct (access_mode t); try done.
+  destruct (type_is_volatile t); try done.
+  destruct p; try done.
+  if_tac; try done.
+  iIntros "(% & H)".
+  destruct (eq_dec v Vundef).
+  - subst; iRight; eauto.
+  - iLeft; iFrame; auto.
+Qed.
+
+Lemma mapsto_eq: forall sh t p v, v ≠ Vundef -> mapsto_memory_block.mapsto sh t p v = mapsto sh t p v.
+Proof.
+  intros; rewrite /mapsto /mapsto_memory_block.mapsto.
+  destruct (access_mode t); try done.
+  destruct (type_is_volatile t); try done.
+  destruct p; try done.
+  if_tac; try done.
+  rewrite (prop_false_andp _ _ H) False_or.
+  do 2 f_equal; apply prop_ext.
+  rewrite /tc_val'; tauto.
+Qed.
+
+Fixpoint memory_block' (sh: share) (n: nat) (b: block) (i: Z) : mpred :=
+  match n with
+  | O => emp
+  | S n' => (if readable_share_dec sh then (b, i) ↦{#sh} VAL Undef
+             else nonlock_permission_bytes sh (b, i) 1)
+         ∗ memory_block' sh n' b (i+1)
+  end.
+
+Definition memory_block'_alt (sh: share) (n: nat) (b: block) (ofs: Z) : mpred :=
+ if readable_share_dec sh
+ then [∗ list] i ∈ seq 0 n, (adr_add (b, ofs) (Z.of_nat i)) ↦{#sh} VAL Undef
+ else nonlock_permission_bytes sh (b,ofs) (Z.of_nat n).
+
+Lemma memory_block'_eq:
+ forall sh n b i,
+  0 <= i ->
+  Z_of_nat n + i < Ptrofs.modulus ->
+  memory_block' sh n b i ⊣⊢ memory_block'_alt sh n b i.
+Proof.
+  intros.
+  unfold memory_block'_alt.
+  revert i H H0; induction n; intros.
+  + if_tac; reflexivity.
+  + unfold memory_block'; fold memory_block'.
+    rewrite -> (IHn (i+1)) by (rewrite inj_S in H0; lia).
+    if_tac.
+    - simpl; f_equiv.
+      * rewrite /adr_add /= Z.add_0_r //.
+      * rewrite -(fmap_add_seq 1 0) big_sepL_fmap; do 3 f_equiv.
+        rewrite /adr_add /=; do 2 f_equiv; lia.
+    - rewrite -> (nonlock_permission_bytes_split2 1 (Z_of_nat n) (Z.of_nat (S n))) by (try rewrite inj_S; lia); done.
+Qed.
+
+Definition memory_block (sh: share) (n: Z) (v: val) : mpred :=
+ match v with
+ | Vptr b ofs => ⌜Ptrofs.unsigned ofs + n < Ptrofs.modulus⌝ ∧ memory_block' sh (Z.to_nat n) b (Ptrofs.unsigned ofs)
+ | _ => False
+ end.
+
+Lemma memory_block_weaken: forall sh n v, memory_block sh n v ⊢ mapsto_memory_block.memory_block sh n v.
+Proof.
+  intros; rewrite /memory_block /mapsto_memory_block.memory_block.
+  destruct v; try done.
+  iIntros "(% & H)"; iSplit; first done; iStopProof.
+  destruct (zlt n 0).
+  { rewrite Z2Nat_neg //. }
+  rewrite -(Z2Nat.id n) in H; last lia.
+  generalize dependent i; induction (Z.to_nat n); simpl; intros; first done.
+  f_equiv.
+  - rewrite Ptrofs.repr_unsigned /mapsto_memory_block.mapsto_ /mapsto_memory_block.mapsto /=.
+    if_tac.
+    + iIntros "H"; iRight; iSplit; first done.
+      rewrite address_mapsto_undef; iFrame.
+    + iIntros "$"; iPureIntro; split; last done.
+      split; [apply tc_val'_Vundef | apply Z.divide_1_l].
+  - specialize (IHn0 (Ptrofs.add i Ptrofs.one)).
+    rewrite Ptrofs.add_unsigned Ptrofs.unsigned_repr Ptrofs.unsigned_one in IHn0.
+    apply IHn0; lia.
+    { unfold Ptrofs.max_unsigned; pose proof (Ptrofs.unsigned_range i); lia. }
+Qed.
+
+Lemma mapsto__exp_address_mapsto: forall sh t b i_ofs ch,
+  access_mode t = By_value ch ->
+  type_is_volatile t = false ->
+  readable_share sh ->
+  mapsto_ sh t (Vptr b i_ofs) ⊣⊢ ∃ v2' : val, <affine> ⌜tc_val' t v2'⌝ ∗
+            address_mapsto ch v2' sh (b, (Ptrofs.unsigned i_ofs)).
+Proof.
+  intros.
+  unfold mapsto_, mapsto; do 2 f_equiv.
+  rewrite H H0.
+  rewrite -> if_true by auto.
+  apply bi.persistent_and_affinely_sep_l; apply _.
+Qed.
+
+(*Lemma mapsto__memory_block: forall sh b ofs t ch,
+  access_mode t = By_value ch ->
+  type_is_volatile t = false ->
+  (align_chunk ch | Ptrofs.unsigned ofs) ->
+  Ptrofs.unsigned ofs + size_chunk ch < Ptrofs.modulus ->
+  mapsto sh t (Vptr b ofs) Vundef ⊣⊢ memory_block sh (size_chunk ch) (Vptr b ofs).
+Proof.
+  intros.
+  unfold mapsto_, mapsto, memory_block, memory_block'.
+  pose proof (tc_val'_Vundef t).
+  rewrite H H0 (pure_True _ H2) !pure_True // !True_and.
+  if_tac.
+  - iIntros "(% & % & % & % & H)".
+    rewrite address_mapsto_VALspec_range /VALspec_range.
+    forget (Ptrofs.unsigned ofs) as o.
+    clear - H3; iInduction (Z.to_nat (size_chunk ch)) as [|] "IH" forall (o); simpl; first done.
+    rewrite /mapsto_ /mapsto /=.
+    iDestruct "H" as "(H & Hrest)"; iSplitL "H".
+    + Search VALspec_range address_mapsto.
+    Search seq S.
+big_sepL_snoc
+    Search big_opL bi_sep app.
+  if_tac.
+  trans (∃ v : val,
+   if readable_share_dec sh
+   then ⌜tc_val' t v⌝ ∧ address_mapsto ch v sh (b, Ptrofs.unsigned ofs)
+   else
+    ⌜tc_val' t v⌝
+    ∧ nonlock_permission_bytes sh (b, Ptrofs.unsigned ofs) (size_chunk ch)).
+  { do 2 f_equiv.
+    rewrite pure_and (pure_True _ H1) and_True //. }
+  rewrite (pure_True _ H2) True_and.
+  clear.
+  remember (Z.to_nat (size_chunk ch)) as n; generalize dependent ch; induction n; simpl; intros.
+  - 
+  setoid_rewrite bi.pure_and.
+  rewrite memory_block'_eq.
+  2: pose proof Ptrofs.unsigned_range ofs; lia.
+  2: rewrite -> Z2Nat.id by (pose proof size_chunk_pos ch; lia); lia.
+  rewrite bi.pure_True; last done.
+  rewrite bi.True_and.
+  unfold memory_block'_alt; destruct (readable_share_dec sh).
+ * rewrite -> mapsto__exp_address_mapsto with (ch := ch); auto.
+  rewrite -> Z2Nat.id by (pose proof size_chunk_pos ch; lia).
+  rewrite -> VALspec_range_exp_address_mapsto_eq by (exact H1).
+  done.
+ * unfold mapsto_, mapsto.
+  rewrite H H0.
+  rewrite -> if_false by auto.
+  rewrite -> bi.pure_True by (split; [apply tc_val'_Vundef | auto]).
+  rewrite -> Z2Nat.id by (pose proof (size_chunk_pos ch); lia).
+  by rewrite bi.True_and.
+Qed.
+
+Lemma nonreadable_memory_block_mapsto: forall sh b ofs t ch v,
+  ~ readable_share sh ->
+  access_mode t = By_value ch ->
+  type_is_volatile t = false ->
+  (align_chunk ch | Ptrofs.unsigned ofs) ->
+  Ptrofs.unsigned ofs + size_chunk ch < Ptrofs.modulus ->
+  tc_val' t v ->
+  memory_block sh (size_chunk ch) (Vptr b ofs) ⊣⊢ mapsto sh t (Vptr b ofs) v.
+Proof.
+  intros.
+  rewrite -mapsto__memory_block; eauto.
+  rewrite /mapsto_ /mapsto.
+  rewrite H0 H1 !if_false; try done.
+  rewrite !bi.pure_True; try done.
+  split; [apply tc_val'_Vundef | done].
+Qed.*)
+
+Lemma memory_block_eq': forall sh (n : nat) b ofs, 0 <= ofs -> ofs + n <= Ptrofs.max_unsigned ->
+  memory_block' sh n b ofs ⊢ if readable_share_dec sh then VALspec_range n sh (b, ofs)
+    else nonlock_permission_bytes sh (b,ofs) n.
+Proof.
+  intros.
+  rewrite memory_block'_eq /memory_block'_alt //.
+  if_tac; last done.
+  rewrite /VALspec_range Nat2Z.id.
+  apply big_sepL_mono; intros.
+  iIntros "$".
+  { unfold Ptrofs.max_unsigned in *; lia. }
+Qed.
+
+Lemma mapsto__memory_block: forall sh b ofs t ch,
+  access_mode t = By_value ch ->
+  type_is_volatile t = false ->
+  (align_chunk ch | Ptrofs.unsigned ofs) ->
+  memory_block sh (size_chunk ch) (Vptr b ofs) ⊢ mapsto sh t (Vptr b ofs) Vundef.
+Proof.
+  intros.
+  unfold mapsto_, mapsto, memory_block.
+  iIntros "(% & H)".
+  rewrite H H0 memory_block'_eq /memory_block'_alt.
+  if_tac.
+  - iSplit; first by iPureIntro; apply tc_val'_Vundef.
+    rewrite /address_mapsto.
+    iExists (repeat Undef (Z.to_nat (size_chunk ch))); iSplit.
+    + rewrite repeat_length.
+      iPureIntro; split3; try done.
+      pose proof (size_chunk_pos ch).
+      destruct (Z.to_nat (size_chunk ch)) eqn: ?; first lia.
+      rewrite /decode_val /=.
+      destruct ch; done.
+    + rewrite (big_sepL_seq (repeat _ _)) repeat_length.
+      by setoid_rewrite nth_repeat.
+  - rewrite Z2Nat.id; last by pose proof (size_chunk_pos ch); lia.
+    iFrame; iPureIntro; split; last done; split; last done.
+    apply tc_val'_Vundef.
+  - apply Ptrofs.unsigned_range.
+  - rewrite Z2Nat.id; last by pose proof (size_chunk_pos ch); lia.
+    lia.
+Qed.
+
+Lemma mapsto_share_join:
+ forall sh1 sh2 sh t p v,
+   sepalg.join sh1 sh2 sh ->
+   mapsto sh1 t p v ∗ mapsto sh2 t p v ⊣⊢ mapsto sh t p v.
+Proof.
+  intros.
+  unfold mapsto.
+  destruct (access_mode t) eqn:?; try solve [rewrite bi.False_sep; auto].
+  destruct (type_is_volatile t) eqn:?; try solve [rewrite bi.False_sep; auto].
+  destruct p; try solve [rewrite bi.False_sep; auto].
+  destruct (readable_share_dec sh1), (readable_share_dec sh2);
+    try rewrite -> (if_true (readable_share sh)) by (eapply join_sub_readable; [unfold sepalg.join_sub; eauto | auto]).
+  + rewrite sepcon_andp_prop' sepcon_andp_prop assoc andp_dup; f_equiv.
+    rewrite address_mapsto_share_join //.
+  + rewrite sepcon_andp_prop' sepcon_andp_prop assoc -pure_and.
+    rewrite (address_mapsto_align _ _ sh) (and_comm _ (_ ∧ _)) -assoc -pure_and and_comm; f_equiv.
+    rewrite comm nonlock_permission_bytes_address_mapsto_join //.
+    by apply sepalg.join_comm.
+    { f_equiv; tauto. }
+  + rewrite -> (if_true (readable_share sh)) by (eapply join_sub_readable; [unfold sepalg.join_sub; eexists; apply sepalg.join_comm; eauto | auto]).
+    rewrite sepcon_andp_prop' sepcon_andp_prop assoc -pure_and.
+    rewrite (address_mapsto_align _ _ sh) (and_comm _ (_ ∧ _)) -!assoc -pure_and and_comm; f_equiv.
+    rewrite nonlock_permission_bytes_address_mapsto_join //.
+    { f_equiv; tauto. }
+  + rewrite -> if_false by (eapply join_unreadable_shares; eauto).
+    rewrite -(nonlock_permission_bytes_share_join _ _ _ _ _ H); auto.
+    rewrite sepcon_andp_prop' sepcon_andp_prop assoc andp_dup //.
+Qed.
+
+Lemma mapsto_share_joins:
+ forall sh1 sh2 t p v,
+   mapsto sh1 t p v ∗ mapsto sh2 t p v ⊢ ⌜sepalg.joins sh1 sh2⌝.
+Proof.
+  intros.
+  unfold mapsto.
+  iIntros "[H1 H2]".
+  destruct (access_mode t) eqn:?; try done.
+  destruct (type_is_volatile t) eqn:?; try done.
+  destruct p; try done.
+  destruct (readable_share_dec sh1), (readable_share_dec sh2).
+  + iDestruct "H1" as (?) "H1"; iDestruct "H2" as (?) "H2".
+    by iApply (address_mapsto_share_joins with "[$H1 $H2]").
+  + iDestruct "H1" as (?) "H1"; iDestruct "H2" as (?) "H2".
+    iDestruct (nonlock_permission_bytes_address_mapsto_joins with "[$H1 $H2]") as %?; iPureIntro; by apply psepalg.joins_comm.
+  + iDestruct "H1" as (?) "H1"; iDestruct "H2" as (?) "H2".
+    by iApply (nonlock_permission_bytes_address_mapsto_joins with "[$H1 $H2]").
+  + iDestruct "H1" as "(% & H1)"; iDestruct "H2" as "(% & H2)".
+    iApply (nonlock_permission_bytes_share_joins with "[$H1 $H2]").
+    apply size_chunk_pos.
+Qed.
+
+Lemma mapsto_mapsto_: forall sh t v v', mapsto sh t v v' ⊢ mapsto_ sh t v.
+Proof. unfold mapsto_; intros; eauto. Qed.
+
+Lemma memory_block_share_joins:
+  forall sh1 sh2 n p, n > 0 ->
+   memory_block sh1 n p ∗ memory_block sh2 n p ⊢ ⌜sepalg.joins sh1 sh2⌝.
+Proof.
+  intros.
+  unfold memory_block.
+  iIntros "[H1 H2]".
+  destruct p; try done.
+  destruct (Z.to_nat n) eqn: Hn; simpl; first lia.
+  iDestruct "H1" as (_) "(H1 & _)"; iDestruct "H2" as (_) "(H2 & _)".
+  if_tac; if_tac; rewrite ?address_mapsto_undef.
+  + by iApply (address_mapsto_share_joins with "[$H1 $H2]").
+  + iDestruct (nonlock_permission_bytes_address_mapsto_joins with "[$H1 $H2]") as %?; iPureIntro; by apply psepalg.joins_comm.
+  + by iApply (nonlock_permission_bytes_address_mapsto_joins with "[H1 $H2]").
+  + by iApply (nonlock_permission_bytes_share_joins with "[$H1 $H2]").
+Qed.
+
+Lemma mapsto_pure_facts: forall sh t p v,
+  mapsto sh t p v ⊢ ⌜(exists ch, access_mode t = By_value ch) /\ isptr p⌝.
+Proof.
+  intros.
+  unfold mapsto.
+  destruct (access_mode t); try iIntros "[]".
+  destruct (type_is_volatile t); try iIntros "[]".
+  destruct p; try iIntros "[]".
+  iIntros "_"; iPureIntro; simpl; eauto.
+Qed.
+
+Lemma mapsto_overlap: forall sh {cs: compspecs} t1 t2 p1 p2 v1 v2
+  (Hsh : sh <> Share.bot), pointer_range_overlap p1 (Ctypes.sizeof t1) p2 (Ctypes.sizeof t2) ->
+  mapsto sh t1 p1 v1 ∗ mapsto sh t2 p2 v2 ⊢ False.
+Proof.
+  intros.
+  unfold mapsto.
+  destruct (access_mode t1) eqn:AM1; try iIntros "[[] _]".
+  destruct (access_mode t2) eqn:AM2; try iIntros "[_ []]".
+  destruct (type_is_volatile t1); try iIntros "[[] _]".
+  destruct (type_is_volatile t2); try iIntros "[_ []]".
+  destruct p1; try iIntros "[[] _]".
+  destruct p2; try iIntros "[_ []]".
+  destruct H as (? & ? & H1 & H2 & H); simpl in *; subst.
+  erewrite -> !size_chunk_sizeof in H by eauto.
+  apply range_overlap_comm in H.
+  if_tac.
+  + iIntros "((_ & H1) & (_ & H2))".
+    iApply address_mapsto_overlap; eauto with iFrame.
+  + iIntros "[[% H] [% ?]]".
+    iApply nonlock_permission_bytes_overlap; eauto with iFrame.
+Qed.
+
+Lemma memory_block_overlap: forall sh p1 n1 p2 n2 (Hsh : sh <> Share.bot), pointer_range_overlap p1 n1 p2 n2 -> memory_block sh n1 p1 ∗ memory_block sh n2 p2 ⊢ False.
+Proof.
+  intros.
+  unfold memory_block.
+  destruct p1; try iIntros "[[] _]".
+  destruct p2; try iIntros "[_ []]".
+  iIntros "[[% H] [% H2]]".
+  destruct (pointer_range_overlap_non_zero _ _ _ _ H).
+  destruct H as (? & ? & ? & ? & H%range_overlap_comm); simpl in *; subst.
+  rewrite !memory_block_eq'.
+  if_tac.
+  + iApply (VALspec_range_overlap with "[$H $H2]").
+    apply range_overlap_comm; rewrite !Z2Nat.id //; lia.
+  + iApply (nonlock_permission_bytes_overlap with "[$]"); first done.
+    rewrite !Z2Nat.id; auto; lia.
+  + apply Ptrofs.unsigned_range.
+  + rewrite Z2Nat.id /Ptrofs.max_unsigned; lia.
+  + apply Ptrofs.unsigned_range.
+  + rewrite Z2Nat.id /Ptrofs.max_unsigned; lia.
+Qed.
+
+Lemma mapsto_conflict:
+  forall {cs : compspecs} sh t v v2 v3 (Hsh : sh <> Share.bot),
+  mapsto sh t v v2 ∗ mapsto sh t v v3 ⊢ False.
+Proof.
+  intros.
+  iIntros "[H1 H2]".
+  iDestruct (mapsto_pure_facts with "H1") as %[[??] ?].
+  assert (Ctypes.sizeof t > 0).
+  { destruct t; try discriminate; simpl; try destruct i; try destruct f; try simple_if_tac; lia. }
+  iApply (mapsto_overlap _ (cs := cs) with "[$]"); first done.
+  apply pointer_range_overlap_refl; auto.
+Qed.
+
+Lemma memory_block_conflict: forall sh n m p (Hsh : sh <> Share.bot),
+  0 < n <= Ptrofs.max_unsigned -> 0 < m <= Ptrofs.max_unsigned ->
+  memory_block sh n p ∗ memory_block sh m p ⊢ False.
+Proof.
+  intros.
+  destruct p; try iIntros "[[] _]".
+  apply memory_block_overlap; first done.
+  exists (b, Ptrofs.unsigned i), (b, Ptrofs.unsigned i); split3; try done.
+  exists (b, Ptrofs.unsigned i).
+  simpl; repeat split; auto; lia.
+Qed.
+
+Lemma memory_block_non_pos_Vptr: forall sh n b z, n <= 0 -> memory_block sh n (Vptr b z) = emp.
+Proof.
+  intros. unfold memory_block.
+  rewrite -> Z_to_nat_neg by auto.
+  unfold memory_block'.
+  rewrite prop_true_andp //.
+  pose proof Ptrofs.unsigned_range z. lia.
+Qed.
+
+Lemma memory_block_zero_Vptr: forall sh b z, memory_block sh 0 (Vptr b z) = emp.
+Proof.
+  intros; apply memory_block_non_pos_Vptr.
+  lia.
+Qed.
+
+Lemma memory_block'_split:
+  forall sh b ofs i j,
+   0 <= i <= j ->
+    j <= j+ofs < Ptrofs.modulus ->
+   memory_block' sh (Z.to_nat j) b ofs ⊣⊢
+      memory_block' sh (Z.to_nat i) b ofs ∗ memory_block' sh (Z.to_nat (j-i)) b (ofs+i).
+Proof.
+  intros.
+  rewrite !memory_block'_eq; try rewrite Z2Nat.id; try lia.
+  rewrite /memory_block'_alt.
+  rewrite -> !Z2Nat.id by lia.
+  if_tac.
+  + replace (Z.to_nat j) with (Z.to_nat i + Z.to_nat (j - i))%nat by lia.
+    rewrite seq_app big_sepL_app; f_equiv.
+    replace (0 + Z.to_nat i)%nat with (Z.to_nat i + 0)%nat by lia.
+    rewrite -fmap_add_seq big_sepL_fmap; do 3 f_equiv.
+    rewrite /adr_add /=; do 2 f_equiv; lia.
+  + apply nonlock_permission_bytes_split2; lia.
+Qed.
+
+Lemma memory_block_split:
+  forall (sh : share) (b : block) (ofs n m : Z),
+  0 <= n ->
+  0 <= m ->
+  n + m <= n + m + ofs < Ptrofs.modulus ->
+  memory_block sh (n + m) (Vptr b (Ptrofs.repr ofs)) ⊣⊢
+  memory_block sh n (Vptr b (Ptrofs.repr ofs)) ∗
+  memory_block sh m (Vptr b (Ptrofs.repr (ofs + n))).
+Proof.
+  intros.
+  unfold memory_block.
+  rewrite -> memory_block'_split with (i := n); [| lia |].
+  2:{
+    pose proof Ptrofs.unsigned_range (Ptrofs.repr ofs).
+    pose proof Ptrofs.unsigned_repr_eq ofs.
+    assert (ofs mod Ptrofs.modulus <= ofs) by (apply Z.mod_le; lia).
+    lia.
+  } 
+  replace (n + m - n) with m by lia.
+  replace (memory_block' sh (Z.to_nat m) b (Ptrofs.unsigned (Ptrofs.repr ofs) + n)) with
+    (memory_block' sh (Z.to_nat m) b (Ptrofs.unsigned (Ptrofs.repr (ofs + n)))).
+  2: {
+    destruct (zeq m 0).
+    + subst. reflexivity.
+    + assert (ofs + n < Ptrofs.modulus) by lia.
+      rewrite -> !Ptrofs.unsigned_repr by (unfold Ptrofs.max_unsigned; lia).
+      reflexivity.
+  }
+  iSplit.
+  + iIntros "(% & $ & $)"; iPureIntro; repeat (split; auto); try lia.
+    rewrite Ptrofs.unsigned_repr_eq.
+    assert ((ofs + n) mod Ptrofs.modulus <= ofs + n) by (apply Z.mod_le; lia).
+    lia.
+  + iIntros "[[% $] [% $]]"; iPureIntro; repeat (split; auto); try lia.
+    rewrite Ptrofs.unsigned_repr_eq.
+    assert (ofs mod Ptrofs.modulus <= ofs) by (apply Z.mod_le; lia).
+    lia.
+Qed.
+
+Lemma memory_block_share_join:
+  forall sh1 sh2 sh n p,
+   sepalg.join sh1 sh2 sh ->
+   memory_block sh1 n p ∗ memory_block sh2 n p ⊣⊢ memory_block sh n p.
+Proof.
+  intros.
+  destruct p; try solve [unfold memory_block; rewrite bi.False_sep; auto].
+  destruct (zle 0 n).
+  2:{
+    rewrite -> !memory_block_non_pos_Vptr by lia.
+    by rewrite left_id.
+  }
+  unfold memory_block.
+  destruct (zlt (Ptrofs.unsigned i + n) Ptrofs.modulus).
+  + rewrite -> bi.pure_True by auto.
+    rewrite !bi.True_and.
+    repeat (rewrite memory_block'_eq; [| pose proof Ptrofs.unsigned_range i; lia | rewrite Z2Nat.id; lia]).
+    unfold memory_block'_alt.
+    destruct (readable_share_dec sh1), (readable_share_dec sh2).
+    - rewrite -> if_true by (eapply readable_share_join; eauto).
+      rewrite -big_sepL_sep; do 3 f_equiv.
+      rewrite slice.mapsto_share_join //.
+    - rewrite -> if_true by (eapply readable_share_join; eauto).
+      rewrite /nonlock_permission_bytes Nat2Z.id -big_sepL_sep; do 3 f_equiv.
+      rewrite if_false // mapsto_mapsto_no_share_join //.
+    - rewrite -> if_true by (eapply readable_share_join; eauto).
+      rewrite /nonlock_permission_bytes Nat2Z.id -big_sepL_sep; do 3 f_equiv.
+      rewrite if_false // comm mapsto_mapsto_no_share_join //.
+      by apply sepalg.join_comm.
+    - rewrite if_false.
+      * apply nonlock_permission_bytes_share_join; auto.
+      * eapply join_unreadable_shares; eauto.
+  + rewrite -> bi.pure_False by auto.
+    by rewrite !bi.False_and bi.False_sep.
+Qed.
+
+Lemma mapsto_pointer_void:
+  forall sh t a, 
+   eqb_type (Tpointer t a) int_or_ptr_type = false ->
+   eqb_type (Tpointer Tvoid a) int_or_ptr_type = false ->
+   mapsto sh (Tpointer t a) = mapsto sh (Tpointer Tvoid a).
+Proof.
+intros.
+unfold mapsto.
+extensionality v1 v2.
+unfold tc_val', tc_val. rewrite H H0.
+reflexivity.
+Qed.
+
+Lemma mapsto_core_load: forall t ch sh v b o, access_mode t = By_value ch -> readable_share sh ->
+  mapsto sh t (Vptr b o) v ⊢ core_load ch (b, Ptrofs.unsigned o) v.
+Proof.
+  unfold mapsto.
+  intros; rewrite H.
+  iIntros "H".
+  destruct (type_is_volatile t); try done.
+  rewrite -> if_true by auto.
+  iDestruct "H" as (?) "H"; by iApply (assert_lemmas.mapsto_core_load with "H").
+Qed.
+
+(* Timeless *)
+Lemma nonlock_permission_bytes_timeless sh l n : n > 0 -> Timeless (nonlock_permission_bytes sh l n).
+Proof.
+  intros; rewrite /nonlock_permission_bytes.
+  apply big_sepL_timeless'.
+  intros; if_tac; try apply _.
+  apply bi.exist_timeless; intros; apply bi.and_timeless; try apply _.
+  apply gen_heap.mapsto_timeless; done.
+  { destruct (Z.to_nat _) eqn: Hn; try done; lia. }
+Qed.
+
+Global Instance mapsto_timeless sh t v1 v2 : Timeless (mapsto sh t v1 v2).
+Proof.
+  rewrite /mapsto.
+  destruct (access_mode t); try apply _.
+  destruct (type_is_volatile t); try apply _.
+  destruct v1; try apply _.
+  if_tac; try apply _.
+  apply bi.and_timeless; first apply _.
+  apply nonlock_permission_bytes_timeless, size_chunk_pos.
+Qed.
+
+Lemma memory_block'_timeless sh n b o : (n > 0)%nat -> Timeless (memory_block' sh n b o).
+Proof.
+  revert o; induction n; simpl; first lia; intros.
+  destruct (gt_dec n O).
+  - apply bi.sep_timeless; [|eauto].
+    if_tac; first apply _.
+    by apply nonlock_permission_bytes_timeless.
+  - replace n with O by lia; rewrite bi.sep_emp.
+    if_tac; first apply _.
+    by apply nonlock_permission_bytes_timeless.
+Qed.
+
+Lemma memory_block_timeless sh z p : z > 0 -> Timeless (memory_block sh z p).
+Proof.
+  intros.
+  destruct p; simpl; try apply _.
+  apply bi.and_timeless; first apply _.
+  apply memory_block'_timeless; lia.
+Qed.
+
+(* valid_pointer *)
+Lemma mapsto_valid_pointer1: forall {cs: compspecs} sh t p v i,
+  match p with Vptr _ ofs => Ptrofs.unsigned ofs + i < Ptrofs.modulus | _ => True end ->
+  0 <= i < sizeof t ->
+  sh <> Share.bot ->
+  mapsto sh t p v ⊢ valid_pointer (offset_val i p).
+Proof.
+  intros; iIntros "H".
+  unfold mapsto.
+  destruct (access_mode t) eqn:?H; auto.
+  destruct (type_is_volatile t); auto.
+  destruct p; auto.
+  simpl in H; unfold sizeof in *.
+  erewrite size_chunk_sizeof in H0 by eauto.
+  pose proof (Ptrofs.unsigned_range i0).
+  destruct (readable_share_dec sh).
+  + iDestruct "H" as "(% & H)"; iApply (address_mapsto_valid_pointer1 with "H"); rewrite ?Ptrofs.unsigned_repr /Ptrofs.max_unsigned; lia.
+  + iDestruct "H" as "[% H]"; iApply (nonlock_permission_bytes_valid_pointer1 with "H"); last done; rewrite ?Ptrofs.unsigned_repr /Ptrofs.max_unsigned; lia.
+Qed.
+
+Lemma mapsto_valid_pointer: forall {cs: compspecs} sh t p v i,
+  size_compatible t p -> 
+  0 <= i < sizeof t ->
+  sh <> Share.bot ->
+  mapsto sh t p v ⊢ valid_pointer (offset_val i p).
+Proof.
+  intros; apply mapsto_valid_pointer1; auto.
+  destruct p; auto; simpl in H; lia.
+Qed.
+
+Lemma memory_block_valid_pointer: forall {cs: compspecs} sh n p i,
+  0 <= i < n ->
+  sh <> Share.bot ->
+  memory_block sh n p ⊢ valid_pointer (offset_val i p).
+Proof.
+  intros.
+  unfold memory_block.
+  destruct p; auto.
+  iIntros "[% H]".
+  pose proof Ptrofs.unsigned_range i0.
+  rewrite -> memory_block'_eq by (rewrite ?Z2Nat.id; lia).
+  unfold memory_block'_alt.
+  rewrite -> Z2Nat.id by lia.
+  destruct (readable_share_dec sh).
+  + rewrite (big_sepL_lookup_acc _ _ (Z.to_nat i)); last by apply lookup_seq; split; try lia.
+    iDestruct "H" as "(H & _)"; rewrite /adr_add /=.
+    assert (0 <= i <= Ptrofs.max_unsigned) by (unfold Ptrofs.max_unsigned; lia).
+    rewrite Ptrofs.add_unsigned !Ptrofs.unsigned_repr //.
+    rewrite Z.add_0_r Z2Nat.id; last lia.
+    iLeft; iFrame.
+    { unfold Ptrofs.max_unsigned; lia. }
+  + iApply (nonlock_permission_bytes_valid_pointer with "H"); last done; rewrite ?Ptrofs.unsigned_repr /Ptrofs.max_unsigned; lia.
+Qed.
+
+Lemma memory_block_weak_valid_pointer: forall {cs: compspecs} sh n p i,
+  0 <= i <= n -> 0 < n ->
+  sh <> Share.bot ->
+  memory_block sh n p ⊢ weak_valid_pointer (offset_val i p).
+Proof.
+  intros. unfold memory_block. destruct p; auto. iIntros "[% H]".
+  pose proof Ptrofs.unsigned_range i0. rewrite -> memory_block'_eq by (rewrite ?Z2Nat.id; lia).
+  unfold memory_block'_alt.
+  rewrite -> Z2Nat.id by lia. destruct (readable_share_dec sh).
+  + destruct (decide (i = n)).
+    * rewrite (big_sepL_lookup_acc _ _ (Z.to_nat (i - 1))); last by apply lookup_seq; split; try lia.
+      iDestruct "H" as "(H & _)"; rewrite /adr_add /=.
+      assert (0 <= i <= Ptrofs.max_unsigned) by (unfold Ptrofs.max_unsigned; lia).
+      rewrite Ptrofs.add_unsigned !Ptrofs.unsigned_repr //.
+      iRight; simpl.
+      replace (Ptrofs.unsigned (Ptrofs.repr (Ptrofs.unsigned i0 + i)) + -1) with (Ptrofs.unsigned i0 + Z.to_nat (i - 1)).
+      iLeft; iFrame.
+      { rewrite Ptrofs.unsigned_repr; unfold Ptrofs.max_unsigned; lia. }
+    * rewrite (big_sepL_lookup_acc _ _ (Z.to_nat i)); last by apply lookup_seq; split; try lia.
+      iDestruct "H" as "(H & _)"; rewrite /adr_add /=.
+      iLeft; simpl.
+      assert (0 <= i <= Ptrofs.max_unsigned) by (unfold Ptrofs.max_unsigned; lia).
+      rewrite Ptrofs.add_unsigned !Ptrofs.unsigned_repr //.
+      rewrite Z.add_0_r Z2Nat.id; last lia.
+      iLeft; iFrame.
+      { unfold Ptrofs.max_unsigned; lia. }
+  + iApply (nonlock_permission_bytes_weak_valid_pointer with "H"); last done; rewrite ?Ptrofs.unsigned_repr /Ptrofs.max_unsigned; lia.
+Qed.
+
+End mpred.
